Prove normal_form red -> lang_nf

Lang/NormalForm.v
@@ -22,6 +22,56 @@ Inductive lang_nf {V : Set} : expr V -> Prop :=
   | lang_nf_app : forall C v1 v2, non_lam v1      -> lang_nf (C[ e_app v1 v2 ]ᵢ)
   | lang_nf_do : forall C v l, ~IctxHandlesOp C l -> lang_nf (C[ e_do l v ]ᵢ).
 
+Inductive predex {V : Set} : expr V -> Prop :=
+  | predex_add : forall v1 v2, predex (e_add v1 v2)
+  | predex_app : forall v1 v2, predex (e_app v1 v2)
+  | predex_let : forall (v : value V) e, predex (e_let v e)
+  | predex_handle_ret : forall (v : value V) h, predex (e_handle v h)
+  | predex_handle_do : forall h (C : o_ctx V) l v,
+      ~OctxHandlesOp C l -> HandlesOp h l ->
+      predex (e_handle (C [ e_do l v ]ₒ) h).
+
+Hint Constructors predex : core.
+
+Lemma lang_decomposition_o :
+  forall {V : Set} (e : expr V),
+    (exists (v : value V), e = v)
+    \/ (exists C p, e = C[p]ₒ /\ predex p)
+    \/ (exists C l v, e = C[ e_do l v ]ₒ /\ ~OctxHandlesOp C l).
+Proof.
+  intros. induction e.
+  - eauto.
+  - right. left. exists o_ctx_hole. simpl. eauto.
+  - right. left. exists o_ctx_hole. simpl. eauto.
+  - destruct IHe1 as [[v ?] | [[C [p [HC Hp]]] | [C [l [v [He1 HC]]]]]]; subst.
+    + right. left. exists o_ctx_hole. simpl. eauto.
+    + right. left. exists (o_ctx_let C e2). simpl. eauto.
+    + right. right. exists (o_ctx_let C e2). simpl. eauto.
+  - right. right. exists o_ctx_hole. simpl. eauto.
+  - destruct IHe as [[v ?] | [[C [p [HC Hp]]] | [C [l [v [He HC]]]]]]; subst.
+    + right. left. exists o_ctx_hole. simpl. eauto.
+    + right. left. exists (o_ctx_handle C h). simpl. eauto.
+    + destruct (HandlesOp_dec h l).
+      * right. left. exists o_ctx_hole. simpl. eauto.
+      * right. right. exists (o_ctx_handle C h). simpl.
+        exists l. exists v. tauto.
+Qed.
+
+Lemma lang_decomposition_i :
+  forall {V : Set} (e : expr V),
+    (exists (v : value V), e = v)
+    \/ (exists C p, e = C[p]ᵢ /\ predex p)
+    \/ (exists C l v, e = C[ e_do l v ]ᵢ /\ ~IctxHandlesOp C l).
+Proof.
+  intros.
+  destruct (lang_decomposition_o e) as [[v ?] | [[C [p [? ?]]] | [C [l [v [? ?]]]]]]; subst.
+  - eauto.
+  - right. left. exists (o_to_i C). exists p. intuition.
+    apply o_plug_bijection.
+  - right. right. exists (o_to_i C). exists l. exists v. split; auto.
+    apply o_plug_bijection.
+Qed.
+
 Theorem canon_let : 
   forall (V : Set) (C : i_ctx V) (v : value V) e,
     C[ e_let v e ]ᵢ = i_ctx_let C e [ v ]ᵢ.
@@ -77,5 +127,29 @@ Proof.
     + inv_redex. inv H0.
     + inv_redex. apply not_i_ctx_handles_op_add_i_distr1 in H0 as [? ?].
       simpl in H0. apply not_or_and in H0 as [? _]. Handles_contra.
-  - admit.
-Admitted.
+  - intros Hnf. destruct (lang_decomposition_i e)
+    as [[v ?] | [[C [p [? Hp]]] | [C [l [v [? ?]]]]]]; subst.
+    + apply lang_nf_val.
+    + inv Hp; unfold normal_form in Hnf.
+      * destruct v1; destruct v2.
+        -- exfalso. apply Hnf. eexists. apply red_context. constructor.
+        -- apply lang_nf_add2. constructor.
+        -- apply lang_nf_add2. constructor.
+        -- apply lang_nf_add1. constructor.
+        -- apply lang_nf_add1. constructor.
+        -- apply lang_nf_add1. constructor.
+        -- apply lang_nf_add1. constructor.
+        -- apply lang_nf_add1. constructor.
+        -- apply lang_nf_add1. constructor.
+      * destruct v1.
+        -- apply lang_nf_app. constructor.
+        -- apply lang_nf_app. constructor.
+        -- exfalso. apply Hnf. eexists. apply red_context. constructor.
+      * exfalso. apply Hnf. eexists. apply red_context. constructor.
+      * exfalso. apply Hnf. eexists. apply red_context. constructor.
+      * exfalso. apply Hnf. destruct H0 as [e He]. eexists.
+        apply red_context. constructor.
+        -- apply He.
+        -- assumption.
+    + apply lang_nf_do. assumption.
+Qed.
